# 高一下补漏

## 极化恒等式

$$
\begin{split}
\begin{align}
  (\boldsymbol a+\boldsymbol b)^2 = \boldsymbol a^2+\boldsymbol b^2+2\boldsymbol a\boldsymbol b\cdots 1\\
  (\boldsymbol a-\boldsymbol b)^2 = \boldsymbol a^2+\boldsymbol b^2-2\boldsymbol a\boldsymbol b\cdots 2\\
  \end{align}\\
  
 \Longrightarrow
 \left\{
 \begin{aligned}
 \boldsymbol a^2+\boldsymbol b^2=\dfrac{(\boldsymbol a+\boldsymbol b)^2}{2}+\dfrac{(\boldsymbol a-\boldsymbol b)^2}{2}\nonumber\\
  
  4\boldsymbol a\boldsymbol b=(\boldsymbol a+\boldsymbol b)^2-(\boldsymbol a-\boldsymbol b)^2\nonumber
\end{aligned}\right.
  \end{split}
$$

## 柯西不等式

$(a^2+b^2)(c^2+d^2)\geq (ac+bd)^2$

> 证明：
> $$\begin{split}
  (a^2+b^2)(c^2+d^2)= a^2c^2+b^2d^2+a^2d^2+b^2c^2\\
  = a^2c^2+2abcd+b^2d^2+a^2d^2-2abcd+b^2c^2\\
  = (ac+bd)^2+(ad-bc)^2
  \geq (ac+bd)^2
\end{split}$$

## 三点共线

$$\begin{aligned}
\lambda (\boldsymbol a-\boldsymbol b)=\boldsymbol b-\boldsymbol c\\
  \Longrightarrow \boldsymbol b=\dfrac{\lambda}{\lambda +1}\boldsymbol a+\dfrac{1}{\lambda +1}\boldsymbol c
\end{aligned}
$$
